backends/lean/Aeneas/Std/Scalar/Ops/Add.lean
@@ -13,10 +13,10 @@ open Result Error Arith ScalarElab WP
 # Addition: Definitions
 -/
 def UScalar.add {ty : UScalarTy} (x y : UScalar ty) : Result (UScalar ty) :=
-  UScalar.tryMk ty (x.val + y.val)
+  UScalar.tryMk ty (x.toNat + y.toNat)
 
 def IScalar.add {ty : IScalarTy} (x y : IScalar ty) : Result (IScalar ty) :=
-  IScalar.tryMk ty (x.val + y.val)
+  IScalar.tryMk ty (x.toInt + y.toInt)
 
 def UScalar.try_add {ty : UScalarTy} (x y : UScalar ty) : Option (UScalar ty) :=
   Option.ofResult (add x y)
@@ -30,6 +30,18 @@ instance {ty} : HCheckedAdd (UScalar ty) (UScalar ty) (Result (UScalar ty)) wher
 instance {ty} : HCheckedAdd (IScalar ty) (IScalar ty) (Result (IScalar ty)) where
   hCheckedAdd x y := IScalar.add x y
 
+instance : HCheckedAdd UInt8   UInt8   (Result UInt8)   := ⟨@UScalar.add .U8⟩
+instance : HCheckedAdd UInt16  UInt16  (Result UInt16)  := ⟨@UScalar.add .U16⟩
+instance : HCheckedAdd UInt32  UInt32  (Result UInt32)  := ⟨@UScalar.add .U32⟩
+instance : HCheckedAdd UInt64  UInt64  (Result UInt64)  := ⟨@UScalar.add .U64⟩
+instance : HCheckedAdd UInt128 UInt128 (Result UInt128) := ⟨@UScalar.add .U128⟩
+instance : HCheckedAdd USize   USize   (Result USize)   := ⟨@UScalar.add .Usize⟩
+instance : HCheckedAdd Int8    Int8    (Result Int8)    := ⟨@IScalar.add .I8⟩
+instance : HCheckedAdd Int16   Int16   (Result Int16)   := ⟨@IScalar.add .I16⟩
+instance : HCheckedAdd Int32   Int32   (Result Int32)   := ⟨@IScalar.add .I32⟩
+instance : HCheckedAdd Int64   Int64   (Result Int64)   := ⟨@IScalar.add .I64⟩
+instance : HCheckedAdd Int128  Int128  (Result Int128)  := ⟨@IScalar.add .I128⟩
+instance : HCheckedAdd ISize   ISize   (Result ISize)   := ⟨@IScalar.add .Isize⟩
 
 /-!
 # Addition: Theorems
@@ -37,39 +49,38 @@ instance {ty} : HCheckedAdd (IScalar ty) (IScalar ty) (Result (IScalar ty)) wher
 
 theorem UScalar.add_equiv {ty} (x y : UScalar ty) :
   match x +? y with
-  | ok z => x.val + y.val < 2^ty.numBits ∧
-    z.val = x.val + y.val ∧
-    z.bv = x.bv + y.bv
-  | fail _ => ¬ (UScalar.inBounds ty (x.val + y.val))
+  | ok z => x.toNat + y.toNat < 2^ty.numBits ∧
+    z.toNat = x.toNat + y.toNat ∧
+    z.toBitVec = x.toBitVec + y.toBitVec
+  | fail _ => ¬ (UScalar.inBounds ty (x.toNat + y.toNat))
   | _ => ⊥ := by
-  have : x +? y = add x y := by rfl
-  rw [this]
-  simp [add]
+  have heq : (x +? y : Result (UScalar ty)) = UScalar.add x y := rfl
+  rw [heq]
+  simp only [UScalar.add]
   have h := tryMk_eq ty (↑x + ↑y)
-  simp [inBounds] at h
-  split at h <;> simp_all
-  zify; simp
-  zify at h
-  have := @Int.emod_eq_of_lt (x.val + y.val) (2^ty.numBits) (by omega) (by omega)
-  simp [*]
+  split at h <;> simp_all [inBounds, max]
+  apply BitVec.toNat_inj.mp
+  simp only [UScalar.toBitVec_toNat, BitVec.toNat_add]
+  rw [Nat.mod_eq_of_lt (by omega)]
+  omega
 
 theorem IScalar.add_equiv {ty} (x y : IScalar ty) :
   match x +? y with
   | ok z =>
-    IScalar.inBounds ty (x.val + y.val) ∧
-    z.val = x.val + y.val ∧
-    z.bv = x.bv + y.bv
-  | fail _ => ¬ (IScalar.inBounds ty (x.val + y.val))
+    IScalar.inBounds ty (x.toInt + y.toInt) ∧
+    z.toInt = x.toInt + y.toInt ∧
+    z.toBitVec = x.toBitVec + y.toBitVec
+  | fail _ => ¬ (IScalar.inBounds ty (x.toInt + y.toInt))
   | _ => ⊥ := by
-  have : x +? y = add x y := by rfl
-  rw [this]
-  simp [add]
+  have heq : (x +? y : Result (IScalar ty)) = IScalar.add x y := rfl
+  rw [heq]
+  simp [IScalar.add]
   have h := tryMk_eq ty (↑x + ↑y)
   simp [inBounds] at h
   split at h <;> simp_all
   apply BitVec.eq_of_toInt_eq
   simp
-  have := bmod_pow_numBits_eq_of_lt ty (x.val + y.val) (by omega) (by omega)
+  have := bmod_pow_numBits_eq_of_lt ty (x.toInt + y.toInt) (by omega) (by omega)
   simp [*]
 
 /-!
@@ -80,7 +91,7 @@ integers and bit-vectors.
 /-- Generic theorem - shouldn't be used much -/
 theorem UScalar.add_bv_spec {ty} {x y : UScalar ty}
   (hmax : ↑x + ↑y ≤ UScalar.max ty) :
-  x +? y ⦃ z => (↑z : Nat) = ↑x + ↑y ∧ z.bv = x.bv + y.bv ⦄ := by
+  x +? y ⦃ z => z.toNat = ↑x + ↑y ∧ z.toBitVec = x.toBitVec + y.toBitVec ⦄ := by
   have h := @add_equiv ty x y
   split at h <;> simp_all [max]
   have : 0 < 2^ty.numBits := by simp
@@ -90,18 +101,18 @@ theorem UScalar.add_bv_spec {ty} {x y : UScalar ty}
 theorem IScalar.add_bv_spec {ty}  {x y : IScalar ty}
   (hmin : IScalar.min ty ≤ ↑x + ↑y)
   (hmax : ↑x + ↑y ≤ IScalar.max ty) :
-  x +? y ⦃ z => (↑z : Int) = ↑x + ↑y ∧ z.bv = x.bv + y.bv ⦄ := by
+  x +? y ⦃ z => z.toInt = ↑x + ↑y ∧ z.toBitVec = x.toBitVec + y.toBitVec ⦄ := by
   have h := @add_equiv ty x y
   split at h <;> simp_all [min, max]
   omega
 
-uscalar theorem «%S».add_bv_spec {x y : «%S»} (hmax : x.val + y.val ≤ «%S».max) :
-  x +? y ⦃ z => (↑z : Nat) = ↑x + ↑y ∧ z.bv = x.bv + y.bv ⦄ :=
+uscalar theorem «%S».add_bv_spec {x y : «%S»} (hmax : x.toNat + y.toNat ≤ «%S».max) :
+  x +? y ⦃ z => z.toNat = ↑x + ↑y ∧ z.toBitVec = x.toBitVec + y.toBitVec ⦄ :=
   UScalar.add_bv_spec (by scalar_tac)
 
 iscalar theorem «%S».add_bv_spec {x y : «%S»}
   (hmin : «%S».min ≤ ↑x + ↑y) (hmax : ↑x + ↑y ≤ «%S».max) :
-  x +? y ⦃ z => (↑z : Int) = ↑x + ↑y ∧ z.bv = x.bv + y.bv ⦄ :=
+  x +? y ⦃ z => z.toInt = ↑x + ↑y ∧ z.toBitVec = x.toBitVec + y.toBitVec ⦄ :=
   IScalar.add_bv_spec (by scalar_tac) (by scalar_tac)
 
 /-!
@@ -114,7 +125,7 @@ only integers. Those are the most common to use, so we mark them with the
 @[step]
 theorem UScalar.add_spec {ty} {x y : UScalar ty}
   (hmax : ↑x + ↑y ≤ UScalar.max ty) :
-  x +? y ⦃ z => (↑z : Nat) = ↑x + ↑y ⦄ := by
+  x +? y ⦃ z => z.toNat = ↑x + ↑y ⦄ := by
   have h := @add_equiv ty x y
   split at h <;> simp_all [max]
   have : 0 < 2^ty.numBits := by simp
@@ -125,12 +136,12 @@ theorem UScalar.add_spec {ty} {x y : UScalar ty}
 theorem IScalar.add_spec {ty} {x y : IScalar ty}
   (hmin : IScalar.min ty ≤ ↑x + ↑y)
   (hmax : ↑x + ↑y ≤ IScalar.max ty) :
-  x +? y ⦃ z => (↑z : Int) = ↑x + ↑y ⦄ := by
+  x +? y ⦃ z => z.toInt = ↑x + ↑y ⦄ := by
   have h := @add_equiv ty x y
   split at h <;> simp_all [min, max]
   omega
 
-uscalar @[step] theorem «%S».add_spec {x y : «%S»} (hmax : x.val + y.val ≤ «%S».max) :
+uscalar @[step] theorem «%S».add_spec {x y : «%S»} (hmax : x.toNat + y.toNat ≤ «%S».max) :
   x +? y ⦃ z => (↑z : Nat) = ↑x + ↑y ⦄ :=
   UScalar.add_spec (by scalar_tac)
 
