backends/lean/Aeneas/Std/Scalar/Ops/Rem.lean
@@ -13,10 +13,10 @@ open Result Error Arith ScalarElab WP
 # Remainder: Definitions
 -/
 def UScalar.rem {ty : UScalarTy} (x y : UScalar ty) : Result (UScalar ty) :=
-  if y.val != 0 then ok (UScalar.ofBitVec ty (BitVec.umod (UScalar.toBitVec x) (UScalar.toBitVec y))) else fail divisionByZero
+  if y.toNat != 0 then ok (UScalar.ofBitVec ty (BitVec.umod (UScalar.toBitVec x) (UScalar.toBitVec y))) else fail divisionByZero
 
 def IScalar.rem {ty : IScalarTy} (x y : IScalar ty) : Result (IScalar ty) :=
-  if y.val != 0 then ok (IScalar.ofBitVec ty (BitVec.srem (IScalar.toBitVec x) (IScalar.toBitVec y)))
+  if y.toInt != 0 then ok (IScalar.ofBitVec ty (BitVec.srem (IScalar.toBitVec x) (IScalar.toBitVec y)))
   else fail divisionByZero
 
 def UScalar.try_rem {ty : UScalarTy} (x y : UScalar ty) : Option (UScalar ty) :=
@@ -30,6 +30,19 @@ instance {ty} : HCheckedRem (UScalar ty) (UScalar ty) (Result (UScalar ty)) wher
 
 instance {ty} : HCheckedRem (IScalar ty) (IScalar ty) (Result (IScalar ty)) where
   hCheckedRem x y := IScalar.rem x y
+
+instance : HCheckedRem UInt8   UInt8   (Result UInt8)   := ⟨@UScalar.rem .U8⟩
+instance : HCheckedRem UInt16  UInt16  (Result UInt16)  := ⟨@UScalar.rem .U16⟩
+instance : HCheckedRem UInt32  UInt32  (Result UInt32)  := ⟨@UScalar.rem .U32⟩
+instance : HCheckedRem UInt64  UInt64  (Result UInt64)  := ⟨@UScalar.rem .U64⟩
+instance : HCheckedRem UInt128 UInt128 (Result UInt128) := ⟨@UScalar.rem .U128⟩
+instance : HCheckedRem USize   USize   (Result USize)   := ⟨@UScalar.rem .Usize⟩
+instance : HCheckedRem Int8    Int8    (Result Int8)    := ⟨@IScalar.rem .I8⟩
+instance : HCheckedRem Int16   Int16   (Result Int16)   := ⟨@IScalar.rem .I16⟩
+instance : HCheckedRem Int32   Int32   (Result Int32)   := ⟨@IScalar.rem .I32⟩
+instance : HCheckedRem Int64   Int64   (Result Int64)   := ⟨@IScalar.rem .I64⟩
+instance : HCheckedRem Int128  Int128  (Result Int128)  := ⟨@IScalar.rem .I128⟩
+instance : HCheckedRem ISize   ISize   (Result ISize)   := ⟨@IScalar.rem .Isize⟩
 
 /-!
 # Sanity Checks
@@ -74,28 +87,26 @@ Theorems with a specification which uses integers and bit-vectors
 -/
 
 /-- Generic theorem - shouldn't be used much -/
-theorem UScalar.rem_bv_spec {ty} (x : UScalar ty) {y : UScalar ty} (hzero : y.val ≠ 0) :
-  x %? y ⦃ z => (↑z : Nat) = ↑x % ↑y ∧ z.bv = x.bv % y.bv ⦄ := by
+theorem UScalar.rem_bv_spec {ty} (x : UScalar ty) {y : UScalar ty} (hzero : y.toNat ≠ 0) :
+  x %? y ⦃ z => z.toNat = ↑x % ↑y ∧ z.toBitVec = x.toBitVec % y.toBitVec ⦄ := by
   conv => arg 1; simp [HCheckedRem.hCheckedRem]
-  simp [hzero, rem]
-  simp only [val]
-  simp
+  simp [hzero, UScalar.rem]
 
 /-- Generic theorem - shouldn't be used much -/
-theorem IScalar.rem_bv_spec {ty} (x : IScalar ty) {y : IScalar ty} (hzero : y.val ≠ 0) :
-  x %? y ⦃ z => (↑z : Int) = Int.tmod ↑x ↑y ∧ z.bv = BitVec.srem x.bv y.bv ⦄ := by
+theorem IScalar.rem_bv_spec {ty} (x : IScalar ty) {y : IScalar ty} (hzero : y.toInt ≠ 0) :
+  x %? y ⦃ z => z.toInt = Int.tmod ↑x ↑y ∧ z.toBitVec = BitVec.srem x.toBitVec y.toBitVec ⦄ := by
   conv => arg 1; simp [HCheckedRem.hCheckedRem]
-  simp only [spec_ok, rem, bne_iff_ne, ne_eq, hzero, not_false_eq_true, ↓reduceIte]
-  simp only [val]
-  simp only [BitVec.toInt_srem, bv_toInt_eq, and_true]
+  simp only [spec_ok, IScalar.rem, bne_iff_ne, ne_eq, hzero, not_false_eq_true, ↓reduceIte]
+  simp only [BitVec.toInt_srem, IScalar.toBitVec_toInt, IScalar.ofBitVec_toInt,
+             IScalar.ofBitVec_toBitVec, and_true]
 
 
-uscalar theorem «%S».rem_bv_spec (x : «%S») {y : «%S»} (hnz : y.val ≠ 0) :
-  x %? y ⦃ z => (↑z : Nat) = ↑x % ↑y ∧ z.bv = x.bv % y.bv ⦄ :=
+uscalar theorem «%S».rem_bv_spec (x : «%S») {y : «%S»} (hnz : y.toNat ≠ 0) :
+  x %? y ⦃ z => z.toNat = ↑x % ↑y ∧ z.toBitVec = x.toBitVec % y.toBitVec ⦄ :=
   UScalar.rem_bv_spec x hnz
 
-iscalar theorem «%S».rem_bv_spec (x : «%S») {y : «%S»} (hnz : y.val ≠ 0) :
-  x %? y ⦃ z => (↑z : Int) = Int.tmod ↑x ↑y ∧ z.bv = BitVec.srem x.bv y.bv ⦄ :=
+iscalar theorem «%S».rem_bv_spec (x : «%S») {y : «%S»} (hnz : y.toInt ≠ 0) :
+  x %? y ⦃ z => z.toInt = Int.tmod ↑x ↑y ∧ z.toBitVec = BitVec.srem x.toBitVec y.toBitVec ⦄ :=
   IScalar.rem_bv_spec x hnz
 
 /-!
@@ -103,26 +114,26 @@ Theorems with a specification which only uses integers
 -/
 
 /-- Generic theorem - shouldn't be used much -/
-theorem UScalar.rem_spec {ty} (x : UScalar ty) {y : UScalar ty} (hzero : y.val ≠ 0) :
-  x %? y ⦃ z => (↑z : Nat) = ↑x % ↑y ⦄ := by
+theorem UScalar.rem_spec {ty} (x : UScalar ty) {y : UScalar ty} (hzero : y.toNat ≠ 0) :
+  x %? y ⦃ z => z.toNat = ↑x % ↑y ⦄ := by
   apply spec_mono
   · apply rem_bv_spec x hzero
   · intros x' h
     exact h.1
 
 /-- Generic theorem - shouldn't be used much -/
-theorem IScalar.rem_spec {ty} (x : IScalar ty) {y : IScalar ty} (hzero : y.val ≠ 0) :
-  x %? y ⦃ z => (↑z : Int) = Int.tmod ↑x ↑y ⦄ := by
+theorem IScalar.rem_spec {ty} (x : IScalar ty) {y : IScalar ty} (hzero : y.toInt ≠ 0) :
+  x %? y ⦃ z => z.toInt = Int.tmod ↑x ↑y ⦄ := by
   apply spec_mono
   · apply rem_bv_spec x hzero
   · intros x' h
     exact h.1
 
-uscalar @[step] theorem «%S».rem_spec (x : «%S») {y : «%S»} (hnz : y.val ≠ 0) :
+uscalar @[step] theorem «%S».rem_spec (x : «%S») {y : «%S»} (hnz : y.toNat ≠ 0) :
   x %? y ⦃ z => (↑z : Nat) = ↑x % ↑y ⦄ :=
   UScalar.rem_spec x hnz
 
-iscalar @[step] theorem «%S».rem_spec (x : «%S») {y : «%S»} (hnz : y.val ≠ 0) :
+iscalar @[step] theorem «%S».rem_spec (x : «%S») {y : «%S»} (hnz : y.toInt ≠ 0) :
   x %? y ⦃ z => (↑z : Int) = Int.tmod ↑x ↑y ⦄ :=
   IScalar.rem_spec x hnz
 
