backends/lean/Aeneas/Std/Scalar/Ops/Sub.lean
@@ -14,11 +14,11 @@ open Result Error Arith ScalarElab WP
 -/
 
 def UScalar.sub {ty : UScalarTy} (x y : UScalar ty) : Result (UScalar ty) :=
-  if x.val < y.val then fail .integerOverflow
-  else ok (UScalar.ofBitVec ty (BitVec.ofNat _ (x.val - y.val)))
+  if x.toNat < y.toNat then fail .integerOverflow
+  else ok (UScalar.ofBitVec ty (BitVec.ofNat _ (x.toNat - y.toNat)))
 
 def IScalar.sub {ty : IScalarTy} (x y : IScalar ty) : Result (IScalar ty) :=
-  IScalar.tryMk ty (x.val - y.val)
+  IScalar.tryMk ty (x.toInt - y.toInt)
 
 def UScalar.try_sub {ty : UScalarTy} (x y : UScalar ty) : Option (UScalar ty) :=
   Option.ofResult (sub x y)
@@ -32,6 +32,18 @@ instance {ty} : HCheckedSub (UScalar ty) (UScalar ty) (Result (UScalar ty)) wher
 instance {ty} : HCheckedSub (IScalar ty) (IScalar ty) (Result (IScalar ty)) where
   hCheckedSub x y := IScalar.sub x y
 
+instance : HCheckedSub UInt8   UInt8   (Result UInt8)   := ⟨@UScalar.sub .U8⟩
+instance : HCheckedSub UInt16  UInt16  (Result UInt16)  := ⟨@UScalar.sub .U16⟩
+instance : HCheckedSub UInt32  UInt32  (Result UInt32)  := ⟨@UScalar.sub .U32⟩
+instance : HCheckedSub UInt64  UInt64  (Result UInt64)  := ⟨@UScalar.sub .U64⟩
+instance : HCheckedSub UInt128 UInt128 (Result UInt128) := ⟨@UScalar.sub .U128⟩
+instance : HCheckedSub USize   USize   (Result USize)   := ⟨@UScalar.sub .Usize⟩
+instance : HCheckedSub Int8    Int8    (Result Int8)    := ⟨@IScalar.sub .I8⟩
+instance : HCheckedSub Int16   Int16   (Result Int16)   := ⟨@IScalar.sub .I16⟩
+instance : HCheckedSub Int32   Int32   (Result Int32)   := ⟨@IScalar.sub .I32⟩
+instance : HCheckedSub Int64   Int64   (Result Int64)   := ⟨@IScalar.sub .I64⟩
+instance : HCheckedSub Int128  Int128  (Result Int128)  := ⟨@IScalar.sub .I128⟩
+instance : HCheckedSub ISize   ISize   (Result ISize)   := ⟨@IScalar.sub .Isize⟩
 
 /-!
 # Subtraction: Theorems
@@ -40,39 +52,37 @@ instance {ty} : HCheckedSub (IScalar ty) (IScalar ty) (Result (IScalar ty)) wher
 theorem UScalar.sub_equiv {ty} (x y : UScalar ty) :
   match x -? y with
   | ok z =>
-    y.val ≤ x.val ∧
-    x.val = z.val + y.val ∧
-    z.bv = x.bv - y.bv
-  | fail _ => x.val < y.val
+    y.toNat ≤ x.toNat ∧
+    x.toNat = z.toNat + y.toNat ∧
+    z.toBitVec = x.toBitVec - y.toBitVec
+  | fail _ => x.toNat < y.toNat
   | _ => ⊥ := by
-  have : x -? y = sub x y := by rfl
-  simp [this, sub]
-  dcases h : x.val < y.val <;> simp [h]
+  have : (x -? y : Result (UScalar ty)) = UScalar.sub x y := rfl
+  simp [this, UScalar.sub]
+  dcases h : x.toNat < y.toNat <;> simp [h]
   simp_all
-  simp only [UScalar.val]
-  simp
   split_conjs
-  . have: (x.val - y.val) % 2^ty.numBits = x.val - y.val := by
+  . have: (x.toNat - y.toNat) % 2^ty.numBits = x.toNat - y.toNat := by
       have : 0 < 2^ty.numBits := by simp
       have := x.hBounds
       apply Nat.mod_eq_of_lt; omega
     simp [this]
     omega
   . zify; simp
-    have : (x.val - y.val : Nat) = (x.val : Int) - y.val := by omega
+    have : (x.toNat - y.toNat : Nat) = (x.toNat : Int) - y.toNat := by omega
     rw [this]; clear this
     ring_nf
     rw [Int.add_emod]
-    have : ((2^ty.numBits - y.val) : Nat) % (2^ty.numBits : Int) =
-           (- (y.val : Int)) % (2^ty.numBits : Int) := by
-      have : (2^ty.numBits - y.val : Nat) = (2^ty.numBits : Int) - y.val := by
+    have : ((2^ty.numBits - y.toNat) : Nat) % (2^ty.numBits : Int) =
+           (- (y.toNat : Int)) % (2^ty.numBits : Int) := by
+      have : (2^ty.numBits - y.toNat : Nat) = (2^ty.numBits : Int) - y.toNat := by
         have hBounds := y.hBounds
         zify at *; simp at *
         have : (2^ty.numBits : Nat) = (2^ty.numBits : Int) := by simp
         omega
       rw [this]
       -- TODO: Int.emod_sub_emod not in this version of mathlib
-      have := Int.emod_add_emod (2^ty.numBits) (2^ty.numBits) (-y.val)
+      have := Int.emod_add_emod (2^ty.numBits) (2^ty.numBits) (-y.toNat)
       ring_nf at this
       ring_nf
       rw [← this]
@@ -84,19 +94,19 @@ theorem UScalar.sub_equiv {ty} (x y : UScalar ty) :
 theorem IScalar.sub_equiv {ty} (x y : IScalar ty) :
   match x -? y with
   | ok z =>
-    IScalar.inBounds ty (x.val - y.val) ∧
-    z.val = x.val - y.val ∧
-    z.bv = x.bv - y.bv
-  | fail _ => ¬ (IScalar.inBounds ty (x.val - y.val))
+    IScalar.inBounds ty (x.toInt - y.toInt) ∧
+    z.toInt = x.toInt - y.toInt ∧
+    z.toBitVec = x.toBitVec - y.toBitVec
+  | fail _ => ¬ (IScalar.inBounds ty (x.toInt - y.toInt))
   | _ => ⊥ := by
-  have : x -? y = sub x y := by rfl
-  simp [this, sub]
+  have : (x -? y : Result (IScalar ty)) = IScalar.sub x y := rfl
+  simp [this, IScalar.sub]
   have h := tryMk_eq ty (↑x - ↑y)
   simp [inBounds] at h
   split at h <;> simp_all
   apply BitVec.eq_of_toInt_eq
   simp
-  have := bmod_pow_numBits_eq_of_lt ty (x.val - y.val) (by omega) (by omega)
+  have := bmod_pow_numBits_eq_of_lt ty (x.toInt - y.toInt) (by omega) (by omega)
   simp [*]
 
 /-!
@@ -105,8 +115,8 @@ Theorems with a specification which uses integers and bit-vectors
 
 /- Generic theorem - shouldn't be used much -/
 theorem UScalar.sub_bv_spec {ty} {x y : UScalar ty}
-  (h : y.val ≤ x.val) :
-  x -? y ⦃ z => z.val = x.val - y.val ∧ y.val ≤ x.val ∧ z.bv = x.bv - y.bv ⦄ := by
+  (h : y.toNat ≤ x.toNat) :
+  x -? y ⦃ z => z.toNat = x.toNat - y.toNat ∧ y.toNat ≤ x.toNat ∧ z.toBitVec = x.toBitVec - y.toBitVec ⦄ := by
   have h := @sub_equiv ty x y
   split at h <;> simp_all
   omega
@@ -115,18 +125,18 @@ theorem UScalar.sub_bv_spec {ty} {x y : UScalar ty}
 theorem IScalar.sub_bv_spec {ty} {x y : IScalar ty}
   (hmin : IScalar.min ty ≤ ↑x - ↑y)
   (hmax : ↑x - ↑y ≤ IScalar.max ty) :
-  x -? y ⦃ z => (↑z : Int) = ↑x - ↑y ∧ z.bv = x.bv - y.bv ⦄ := by
+  x -? y ⦃ z => z.toInt = ↑x - ↑y ∧ z.toBitVec = x.toBitVec - y.toBitVec ⦄ := by
   have h := @sub_equiv ty x y
   split at h <;> simp_all [min, max]
   omega
 
-uscalar theorem «%S».sub_bv_spec {x y : «%S»} (h : y.val ≤ x.val) :
-  x -? y ⦃ z => z.val = x.val - y.val ∧ y.val ≤ x.val ∧ z.bv = x.bv - y.bv ⦄ :=
+uscalar theorem «%S».sub_bv_spec {x y : «%S»} (h : y.toNat ≤ x.toNat) :
+  x -? y ⦃ z => z.toNat = x.toNat - y.toNat ∧ y.toNat ≤ x.toNat ∧ z.toBitVec = x.toBitVec - y.toBitVec ⦄ :=
   UScalar.sub_bv_spec h
 
 iscalar theorem «%S».sub_bv_spec {x y : «%S»}
   (hmin : «%S».min ≤ ↑x - ↑y) (hmax : ↑x - ↑y ≤ «%S».max) :
-  x -? y ⦃ z => (↑z : Int) = ↑x - ↑y ∧ z.bv = x.bv - y.bv ⦄ :=
+  x -? y ⦃ z => z.toInt = ↑x - ↑y ∧ z.toBitVec = x.toBitVec - y.toBitVec ⦄ :=
   IScalar.sub_bv_spec (by scalar_tac) (by scalar_tac)
 
 /-!
@@ -136,8 +146,8 @@ Theorems with a specification which only uses integers
 /- Generic theorem - shouldn't be used much -/
 @[step]
 theorem UScalar.sub_spec {ty} {x y : UScalar ty}
-  (h : y.val ≤ x.val) :
-  x -? y ⦃ z => z.val = x.val - y.val ∧ y.val ≤ x.val ⦄ := by
+  (h : y.toNat ≤ x.toNat) :
+  x -? y ⦃ z => z.toNat = x.toNat - y.toNat ∧ y.toNat ≤ x.toNat ⦄ := by
   have h := @sub_equiv ty x y
   split at h <;> simp_all
   omega
@@ -147,13 +157,13 @@ theorem UScalar.sub_spec {ty} {x y : UScalar ty}
 theorem IScalar.sub_spec {ty} {x y : IScalar ty}
   (hmin : IScalar.min ty ≤ ↑x - ↑y)
   (hmax : ↑x - ↑y ≤ IScalar.max ty) :
-  x -? y ⦃ z => (↑z : Int) = ↑x - ↑y ⦄ := by
+  x -? y ⦃ z => z.toInt = ↑x - ↑y ⦄ := by
   have h := @sub_equiv ty x y
   split at h <;> simp_all [min, max]
   omega
 
-uscalar @[step] theorem «%S».sub_spec {x y : «%S»} (h : y.val ≤ x.val) :
-  x -? y ⦃ z => z.val = x.val - y.val ∧ y.val ≤ x.val ⦄ :=
+uscalar @[step] theorem «%S».sub_spec {x y : «%S»} (h : y.toNat ≤ x.toNat) :
+  x -? y ⦃ z => (↑z : Nat) = x.toNat - y.toNat ∧ y.toNat ≤ x.toNat ⦄ :=
   UScalar.sub_spec h
 
 iscalar @[step] theorem «%S».sub_spec {x y : «%S»}
