backends/lean/Aeneas/Std/Scalar/Misc.lean
@@ -18,23 +18,21 @@ theorem bmod_pow_numBits_eq_of_lt (ty : IScalarTy) (x : Int)
 
 /-- We need this lemma to prove the theorems about division and remainder -/
 theorem IScalar.neg_imp_toNat_neg_eq_neg_toInt {ty} (x : IScalar ty) (hNeg : x.toInt < 0):
-  (-x.toBitVec).toNat = -x.toBitVec.toInt := by
-  have hmsb : x.toBitVec.msb = true := by
-    have := @BitVec.msb_eq_toInt _ x.toBitVec
-    simp only [toInt] at hNeg
-    simp only [hNeg] at this
-    apply this
-  have hx := @BitVec.toInt_eq_msb_cond _ x.toBitVec
+  (-(IScalar.toBitVec x)).toNat = -(IScalar.toBitVec x).toInt := by
+  have hmsb : (IScalar.toBitVec x).msb = true := by
+    rw [BitVec.msb_eq_toInt, decide_eq_true_eq]
+    cases ty <;> simp_all [IScalar.toInt, IScalar.toBitVec]
+  have hx := @BitVec.toInt_eq_msb_cond _ (IScalar.toBitVec x)
   simp [hmsb] at hx
 
   have hxNeg : x.toInt < 0 := by
-    have := @BitVec.msb_eq_toInt _ x.toBitVec
+    have := @BitVec.msb_eq_toInt _ (IScalar.toBitVec x)
     simp_all
 
   conv => lhs; simp only [Neg.neg, BitVec.neg]
   simp only [BitVec.toInt_eq_toNat_bmod]
 
-  have hxToNatMod : (x.toBitVec.toNat : Int) % 2^ty.numBits = x.toBitVec.toNat := by
+  have hxToNatMod : ((IScalar.toBitVec x).toNat : Int) % 2^ty.numBits = (IScalar.toBitVec x).toNat := by
     apply Int.emod_eq_of_lt <;> omega
 
   have hPow : (2 ^ ty.numBits + 1 : Int) / 2  = 2^(ty.numBits - 1) := by
@@ -45,8 +43,8 @@ theorem IScalar.neg_imp_toNat_neg_eq_neg_toInt {ty} (x : IScalar ty) (hNeg : x.t
     rw [Int.pow_succ']
     rw [Int.add_ediv_of_dvd_left] <;> simp
 
-  have : ¬ ((x.toBitVec.toNat : Int) % ↑(2 ^ ty.numBits : Nat) < (↑(2 ^ ty.numBits : Nat) + 1) / 2) := by
-    have hIneq := @BitVec.msb_eq_toNat _ x.toBitVec
+  have : ¬ (((IScalar.toBitVec x).toNat : Int) % ↑(2 ^ ty.numBits : Nat) < (↑(2 ^ ty.numBits : Nat) + 1) / 2) := by
+    have hIneq := @BitVec.msb_eq_toNat _ (IScalar.toBitVec x)
     rw [hmsb] at hIneq
     simp at hIneq
     simp
@@ -58,20 +56,20 @@ theorem IScalar.neg_imp_toNat_neg_eq_neg_toInt {ty} (x : IScalar ty) (hNeg : x.t
   rw [Int.bmod_def]
   simp only [this]
   simp
-  have : (2 ^ ty.numBits - x.toBitVec.toNat : Nat) % (2 ^ ty.numBits : Int) =
-         (2^ty.numBits - x.toBitVec.toNat : Nat) := by
+  have : (2 ^ ty.numBits - (IScalar.toBitVec x).toNat : Nat) % (2 ^ ty.numBits : Int) =
+         (2^ty.numBits - (IScalar.toBitVec x).toNat : Nat) := by
     apply Int.emod_eq_of_lt
     . omega
     . have := x.hBounds
-      simp only [toInt] at *
-      have : (2 ^ ty.numBits - x.toBitVec.toNat : Nat) = (2 ^ ty.numBits - x.toBitVec.toNat : Int) := by
+      simp only [IScalar.toInt] at *
+      have : (2 ^ ty.numBits - (IScalar.toBitVec x).toNat : Nat) = (2 ^ ty.numBits - (IScalar.toBitVec x).toNat : Int) := by
         have : (2 ^ ty.numBits : Nat) = (2 ^ ty.numBits : Int) := by simp
         omega
       rw [this]
-      have : x.toBitVec.toNat > 0 := by
+      have : (IScalar.toBitVec x).toNat > 0 := by
         by_contra
-        have hxz : x.toBitVec.toNat = 0 := by omega
-        have : x.toBitVec.toInt = 0 := by
+        have hxz : (IScalar.toBitVec x).toNat = 0 := by omega
+        have : (IScalar.toBitVec x).toInt = 0 := by
           simp only [BitVec.toInt_eq_toNat_bmod, Int.bmod_def, hxz]
           simp [hPow]
         omega
@@ -160,102 +158,104 @@ theorem IScalar.neg_imp_toNat_neg_eq_neg_toInt {ty} (x : IScalar ty) (hNeg : x.t
 -/
 
 theorem UScalar.ofNatCore_bv_lt_equiv {ty} (x y : Nat) (hx) (hy) :
-  (@UScalar.ofNatCore ty x hx).toBitVec < (@UScalar.ofNatCore ty y hy).toBitVec ↔ x < y := by
-  simp only [ofNatCore, UScalar.ofBitVec_toBitVec]
-  have := Nat.mod_eq_of_lt hx
-  have := Nat.mod_eq_of_lt hy
-  simp only [BitVec.lt_ofFin, Fin.mk_lt_mk]
+  (UScalar.toBitVec (@UScalar.ofNatCore ty x hx)) < (UScalar.toBitVec (@UScalar.ofNatCore ty y hy)) ↔ x < y := by
+  simp only [UScalar.ofNatCore, UScalar.toBitVec]
+  cases ty <;> simp [BitVec.lt_ofFin]
 
 @[simp, scalar_tac_simps] theorem U8.val_mod_size_eq (x : U8) : x.toNat % U8.size = x.toNat := by
-  apply Nat.mod_eq_of_lt; scalar_tac_preprocess; exact x.toNat_lt
+  apply Nat.mod_eq_of_lt; scalar_tac
 
 @[simp, scalar_tac_simps] theorem U8.val_mod_size_eq' (x : U8) : x.toNat % 256 = x.toNat := by
-  apply Nat.mod_eq_of_lt; exact x.toNat_lt_size
+  apply Nat.mod_eq_of_lt; scalar_tac
 
-@[simp, scalar_tac_simps] theorem U16.toNat_mod_size_eq (x : U16) : x.toNat % U16.size = x.toNat := by
-  apply Nat.mod_eq_of_lt; scalar_tac_preprocess; exact x.toNat_lt
+@[simp, scalar_tac_simps] theorem U16.val_mod_size_eq (x : U16) : x.toNat % U16.size = x.toNat := by
+  apply Nat.mod_eq_of_lt; scalar_tac
 
-@[simp, scalar_tac_simps] theorem U16.toNat_mod_size_eq' (x : U16) : x.toNat % 65536 = x.toNat := by
-  apply Nat.mod_eq_of_lt; exact x.toNat_lt
+@[simp, scalar_tac_simps] theorem U16.val_mod_size_eq' (x : U16) : x.toNat % 65536 = x.toNat := by
+  apply Nat.mod_eq_of_lt; scalar_tac
 
-@[simp, scalar_tac_simps] theorem U32.toNat_mod_size_eq (x : U32) : x.toNat % U32.size = x.toNat := by
-  apply Nat.mod_eq_of_lt; scalar_tac_preprocess; exact x.toNat_lt
+@[simp, scalar_tac_simps] theorem U32.val_mod_size_eq (x : U32) : x.toNat % U32.size = x.toNat := by
+  apply Nat.mod_eq_of_lt; scalar_tac
 
-@[simp, scalar_tac_simps] theorem U32.toNat_mod_size_eq' (x : U32) : x.toNat % 4294967296 = x.toNat := by
-  apply Nat.mod_eq_of_lt; exact x.toNat_lt
+@[simp, scalar_tac_simps] theorem U32.val_mod_size_eq' (x : U32) : x.toNat % 4294967296 = x.toNat := by
+  apply Nat.mod_eq_of_lt; scalar_tac
 
-@[simp, scalar_tac_simps] theorem U64.toNat_mod_size_eq (x : U64) : x.toNat % U64.size = x.toNat := by
-  apply Nat.mod_eq_of_lt; scalar_tac_preprocess; exact x.toNat_lt
+@[simp, scalar_tac_simps] theorem U64.val_mod_size_eq (x : U64) : x.toNat % U64.size = x.toNat := by
+  apply Nat.mod_eq_of_lt; scalar_tac
 
-@[simp, scalar_tac_simps] theorem U64.toNat_mod_size_eq' (x : U64) : x.toNat % 18446744073709551616 = x.toNat := by
-  apply Nat.mod_eq_of_lt; exact x.toNat_lt
+@[simp, scalar_tac_simps] theorem U64.val_mod_size_eq' (x : U64) : x.toNat % 18446744073709551616 = x.toNat := by
+  apply Nat.mod_eq_of_lt; scalar_tac
 
-@[simp, scalar_tac_simps] theorem U128.toNat_mod_size_eq (x : U128) : x.toNat % U128.size = x.toNat := by
-  apply Nat.mod_eq_of_lt; scalar_tac_preprocess; exact x.toNat_lt
+@[simp, scalar_tac_simps] theorem U128.val_mod_size_eq (x : U128) : x.toNat % U128.size = x.toNat := by
+  apply Nat.mod_eq_of_lt; scalar_tac
 
-@[simp, scalar_tac_simps] theorem U128.toNat_mod_size_eq' (x : U128) : x.toNat % 340282366920938463463374607431768211456 = x.toNat := by
-  apply Nat.mod_eq_of_lt; scalar_tac_preprocess; exact x.toNat_lt
+@[simp, scalar_tac_simps] theorem U128.val_mod_size_eq' (x : U128) : x.toNat % 340282366920938463463374607431768211456 = x.toNat := by
+  apply Nat.mod_eq_of_lt; scalar_tac
 
-@[simp, scalar_tac_simps] theorem Usize.toNat_mod_size_eq (x : Usize) : x.toNat % Usize.size = x.toNat := by
-  apply Nat.mod_eq_of_lt; scalar_tac_preprocess; exact x.toNat_lt_two_pow_numBits
+@[simp, scalar_tac_simps] theorem Usize.val_mod_size_eq (x : Usize) : x.toNat % Usize.size = x.toNat := by
+  apply Nat.mod_eq_of_lt; scalar_tac
 
-@[simp, scalar_tac_simps] theorem U8.toNat_mod_max_eq (x : U8) : x.toNat % (U8.max + 1) = x.toNat := by
-  apply Nat.mod_eq_of_lt; scalar_tac_preprocess; exact x.toNat_lt
+@[simp, scalar_tac_simps] theorem U8.val_mod_max_eq (x : U8) : x.toNat % (U8.max + 1) = x.toNat := by
+  apply Nat.mod_eq_of_lt; scalar_tac
 
-@[simp, scalar_tac_simps] theorem U16.toNat_mod_max_eq (x : U16) : x.toNat % (U16.max + 1) = x.toNat := by
-  apply Nat.mod_eq_of_lt; scalar_tac_preprocess; exact x.toNat_lt
+@[simp, scalar_tac_simps] theorem U16.val_mod_max_eq (x : U16) : x.toNat % (U16.max + 1) = x.toNat := by
+  apply Nat.mod_eq_of_lt; scalar_tac
 
-@[simp, scalar_tac_simps] theorem U32.toNat_mod_max_eq (x : U32) : x.toNat % (U32.max + 1) = x.toNat := by
-  apply Nat.mod_eq_of_lt; scalar_tac_preprocess; exact x.toNat_lt
+@[simp, scalar_tac_simps] theorem U32.val_mod_max_eq (x : U32) : x.toNat % (U32.max + 1) = x.toNat := by
+  apply Nat.mod_eq_of_lt; scalar_tac
 
-@[simp, scalar_tac_simps] theorem U64.toNat_mod_max_eq (x : U64) : x.toNat % (U64.max + 1) = x.toNat := by
-  apply Nat.mod_eq_of_lt; scalar_tac_preprocess; exact x.toNat_lt
+@[simp, scalar_tac_simps] theorem U64.val_mod_max_eq (x : U64) : x.toNat % (U64.max + 1) = x.toNat := by
+  apply Nat.mod_eq_of_lt; scalar_tac
 
-@[simp, scalar_tac_simps] theorem U128.toNat_mod_max_eq (x : U128) : x.toNat % (U128.max + 1) = x.toNat := by
-  apply Nat.mod_eq_of_lt; scalar_tac_preprocess; exact x.toNat_lt
+@[simp, scalar_tac_simps] theorem U128.val_mod_max_eq (x : U128) : x.toNat % (U128.max + 1) = x.toNat := by
+  apply Nat.mod_eq_of_lt; scalar_tac
 
-@[simp, scalar_tac_simps] theorem Usize.toNat_mod_max_eq (x : Usize) : x.toNat % (Usize.max + 1) = x.toNat := by
-  apply Nat.mod_eq_of_lt; scalar_tac_preprocess; exact x.toNat_lt_two_pow_numBits
+@[simp, scalar_tac_simps] theorem Usize.val_mod_max_eq (x : Usize) : x.toNat % (Usize.max + 1) = x.toNat := by
+  apply Nat.mod_eq_of_lt; scalar_tac
 
 @[simp, scalar_tac_simps] theorem I8.val_mod_size_eq (x : I8) : Int.bmod x.toInt I8.size = x.toInt := by
-  simp [size, numBits]
+  simp [size]; apply Int.bmod_pow2_eq_of_inBounds' <;> scalar_tac
 
-@[simp, scalar_tac_simps] theorem I8.toInt_mod_size_eq' (x : I8) : Int.bmod x.toInt 256 = x.toInt := by
+@[simp, scalar_tac_simps] theorem I8.val_mod_size_eq' (x : I8) : Int.bmod x.toInt 256 = x.toInt := by
   simp
 
-@[simp, scalar_tac_simps] theorem I16.toInt_mod_size_eq (x : I16) : Int.bmod x.toInt I16.size = x.toInt := by
-  simp [size, numBits]
+@[simp, scalar_tac_simps] theorem I16.val_mod_size_eq (x : I16) : Int.bmod x.toInt I16.size = x.toInt := by
+  simp [size]; apply Int.bmod_pow2_eq_of_inBounds' <;> scalar_tac
 
-@[simp, scalar_tac_simps] theorem I16.toInt_mod_size_eq' (x : I16) : Int.bmod x.toInt 65536 = x.toInt := by
+@[simp, scalar_tac_simps] theorem I16.val_mod_size_eq' (x : I16) : Int.bmod x.toInt 65536 = x.toInt := by
   simp
 
-@[simp, scalar_tac_simps] theorem I32.toInt_mod_size_eq (x : I32) : Int.bmod x.toInt I32.size = x.toInt := by
-  simp [size, numBits]
+@[simp, scalar_tac_simps] theorem I32.val_mod_size_eq (x : I32) : Int.bmod x.toInt I32.size = x.toInt := by
+  simp [size]; apply Int.bmod_pow2_eq_of_inBounds' <;> scalar_tac
 
-@[simp, scalar_tac_simps] theorem I32.toInt_mod_size_eq' (x : I32) : Int.bmod x.toInt 4294967296 = x.toInt := by
+@[simp, scalar_tac_simps] theorem I32.val_mod_size_eq' (x : I32) : Int.bmod x.toInt 4294967296 = x.toInt := by
   simp
 
-@[simp, scalar_tac_simps] theorem I64.toInt_mod_size_eq (x : I64) : Int.bmod x.toInt I64.size = x.toInt := by
-  simp? [size, numBits]
+@[simp, scalar_tac_simps] theorem I64.val_mod_size_eq (x : I64) : Int.bmod x.toInt I64.size = x.toInt := by
+  simp [size]; apply Int.bmod_pow2_eq_of_inBounds' <;> scalar_tac
 
-@[simp, scalar_tac_simps] theorem I64.toInt_mod_size_eq' (x : I64) : Int.bmod x.toInt 18446744073709551616 = x.toInt := by
+@[simp, scalar_tac_simps] theorem I64.val_mod_size_eq' (x : I64) : Int.bmod x.toInt 18446744073709551616 = x.toInt := by
   simp
 
-@[simp, scalar_tac_simps] theorem I128.toInt_mod_size_eq (x : I128) : Int.bmod x.toInt I128.size = x.toInt := by
-  simp [size, numBits]
+@[simp, scalar_tac_simps] theorem I128.val_mod_size_eq (x : I128) : Int.bmod x.toInt I128.size = x.toInt := by
+  simp [size]; apply Int.bmod_pow2_eq_of_inBounds' <;> scalar_tac
 
-@[simp, scalar_tac_simps] theorem I128.toInt_mod_size_eq' (x : I128) : Int.bmod x.toInt 340282366920938463463374607431768211456 = x.toInt := by
-  simp
+@[simp, scalar_tac_simps] theorem I128.val_mod_size_eq' (x : I128) : Int.bmod x.toInt 340282366920938463463374607431768211456 = x.toInt := by
+  have h := val_mod_size_eq x
+  simp only [I128.size, I128.numBits, IScalarTy.numBits] at h
+  norm_num at h
+  exact h
 
-@[simp, scalar_tac_simps] theorem Isize.toInt_mod_size_eq (x : Isize) : Int.bmod x.toInt Isize.size = x.toInt := by
-  simp [size, numBits]
+@[simp, scalar_tac_simps] theorem Isize.val_mod_size_eq (x : Isize) : Int.bmod x.toInt Isize.size = x.toInt := by
+  simp [size]; apply Int.bmod_pow2_eq_of_inBounds' <;> try scalar_tac
+  simp [numBits]; cases System.Platform.numBits_eq <;> simp [*]
 
 @[simp] theorem U8.val_max_zero_eq (x : U8) : x.toNat ⊔ 0 = x.toNat := by scalar_tac
-@[simp] theorem U16.toNat_max_zero_eq (x : U16) : x.toNat ⊔ 0 = x.toNat := by scalar_tac
-@[simp] theorem U32.toNat_max_zero_eq (x : U32) : x.toNat ⊔ 0 = x.toNat := by scalar_tac
-@[simp] theorem U64.toNat_max_zero_eq (x : U64) : x.toNat ⊔ 0 = x.toNat := by scalar_tac
-@[simp] theorem U128.toNat_max_zero_eq (x : U128) : x.toNat ⊔ 0 = x.toNat := by scalar_tac
-@[simp] theorem Usize.toNat_max_zero_eq (x : Usize) : x.toNat ⊔ 0 = x.toNat := by scalar_tac
+@[simp] theorem U16.val_max_zero_eq (x : U16) : x.toNat ⊔ 0 = x.toNat := by scalar_tac
+@[simp] theorem U32.val_max_zero_eq (x : U32) : x.toNat ⊔ 0 = x.toNat := by scalar_tac
+@[simp] theorem U64.val_max_zero_eq (x : U64) : x.toNat ⊔ 0 = x.toNat := by scalar_tac
+@[simp] theorem U128.val_max_zero_eq (x : U128) : x.toNat ⊔ 0 = x.toNat := by scalar_tac
+@[simp] theorem Usize.val_max_zero_eq (x : Usize) : x.toNat ⊔ 0 = x.toNat := by scalar_tac
 
 
 end Aeneas.Std
