backends/lean/Aeneas/Tactic/Solver/BvTac/BvTac.lean
@@ -127,57 +127,57 @@ elab "bv_tac" config:Parser.Tactic.optConfig n:(colGt term)? : tactic =>
 -/
 open Std
 
-example (x y : U8) (h : x.val ≤ y.val) : x.bv ≤ y.bv := by
+example (x y : U8) (h : x.toNat ≤ y.toNat) : x.toBitVec ≤ y.toBitVec := by
   bv_tac
 
-example (x : U32) (h : x.val < 3329) : x.bv % 3329#32 = x.bv := by
+example (x : U32) (h : x.toNat < 3329) : x.toBitVec % 3329#32 = x.toBitVec := by
   bv_tac
 
 /- Checking parsing -/
-example (x : U32) (h : x.val < 3329) : x.bv % 3329#32 = x.bv ∧ True := by
+example (x : U32) (h : x.toNat < 3329) : x.toBitVec % 3329#32 = x.toBitVec ∧ True := by
   constructor
   bv_tac
   simp
 
 /- Checking parsing -/
-example (x : U32) (h : x.val < 3329) : x.bv % 3329#32 = x.bv ∧ True := by
+example (x : U32) (h : x.toNat < 3329) : x.toBitVec % 3329#32 = x.toBitVec ∧ True := by
   constructor
   bv_tac 32
   simp
 
 /- Checking parsing -/
-example (x : U32) (h : x.val < 3329) : x.bv % 3329#32 = x.bv ∧ True := by
+example (x : U32) (h : x.toNat < 3329) : x.toBitVec % 3329#32 = x.toBitVec ∧ True := by
   constructor
   bv_tac 32; simp
 
 example
   (a : U32)
   (b : U32)
-  (ha : a.val < 3329)
-  (hb : b.val < 3329)
+  (ha : a.toNat < 3329)
+  (hb : b.toNat < 3329)
   (c1 : U32)
-  (_ : c1.bv = a.bv + b.bv)
+  (_ : c1.toBitVec = a.toBitVec + b.toBitVec)
   (c2 : U32)
-  (hc2 : c2 = core.num.U32.wrapping_sub c1 3329#u32)
+  (hc2 : c2.toBitVec = c1.toBitVec - 3329#32)
   (c3 : U32)
-  (hc3 : c3.bv = c2.bv >>> 16#i32.toNat)
-  (_ : ¬c3 = 0#u32) :
-  c3 = 65535#u32
+  (hc3 : c3.toBitVec = c2.toBitVec >>> 16)
+  (_ : c3.toBitVec ≠ 0#32) :
+  c3.toBitVec = 65535#32
   := by
   bv_tac
 
 example
   (a : U32)
   (b : U32)
-  (ha : a.val < 3329)
-  (hb : b.val < 3329)
+  (ha : a.toNat < 3329)
+  (hb : b.toNat < 3329)
   (c1 : U32)
-  (_ : c1.bv = a.bv + b.bv)
+  (_ : c1.toBitVec = a.toBitVec + b.toBitVec)
   (c2 : U32)
-  (_ : c2 = core.num.U32.wrapping_sub c1 3329#u32)
+  (_ : c2.toBitVec = c1.toBitVec - 3329#32)
   (c3 : U32)
-  (_ : c3.bv = c2.bv >>> 16#i32.toNat) :
-  (c1.bv - 3329#32 + (3329#32 &&& c3.bv)) % 3329#32 = (a.bv + b.bv) % 3329#32
+  (_ : c3.toBitVec = c2.toBitVec >>> 16) :
+  (c1.toBitVec - 3329#32 + (3329#32 &&& c3.toBitVec)) % 3329#32 = (a.toBitVec + b.toBitVec) % 3329#32
   := by
   bv_tac
 
@@ -185,12 +185,12 @@ example
   (a : U32)
   (b : U32)
   (c1 : U32)
-  (hc1 : c1 = core.num.U32.wrapping_sub a b)
+  (hc1 : c1.toBitVec = a.toBitVec - b.toBitVec)
   (c2 : U32)
-  (hc2 : c2.bv = c1.bv >>> 16#i32.toNat)
+  (hc2 : c2.toBitVec = c1.toBitVec >>> 16)
   (h : (↑a : ℕ) < 6658 ∧ (↑b : ℕ) = 3329)
-  (_ : ¬c2 = 0#u32) :
-  c2 = 65535#u32
+  (_ : c2.toBitVec ≠ 0#32) :
+  c2.toBitVec = 65535#32
   := by
   bv_tac
 
@@ -201,15 +201,14 @@ example
   (ha : (↑a : ℕ) < (↑b : ℕ) + 3329)
   (hb : (↑b : ℕ) ≤ 3329)
   (c1 : U32)
-  (hc1 : c1 = core.num.U32.wrapping_sub a b)
+  (hc1 : c1.toBitVec = a.toBitVec - b.toBitVec)
   (c2 : U32)
-  (hc2 : c2.bv = c1.bv >>> 16)
+  (hc2 : c2.toBitVec = c1.toBitVec >>> 16)
   (c3 : U32)
-  (hc3_1 : (↑c3 : ℕ) = (↑(3329#u32 &&& c2) : ℕ))
-  (_ : c3.bv = 3329#32 &&& c2.bv)
+  (_ : c3.toBitVec = 3329#32 &&& c2.toBitVec)
   (c4 : U32)
-  (hc3 : c4 = core.num.U32.wrapping_add c1 c3) :
-  c4.bv % 3329#32 = (a.bv + 3329#32 - b.bv) % 3329#32 ∧ c4.bv < 3329#32
+  (hc3 : c4.toBitVec = c1.toBitVec + c3.toBitVec) :
+  c4.toBitVec % 3329#32 = (a.toBitVec + 3329#32 - b.toBitVec) % 3329#32 ∧ c4.toBitVec < 3329#32
   := by
   bv_tac
 
@@ -220,42 +219,41 @@ example
   (hb : (↑b : ℕ) < 3329)
   (c1 : U32)
   (hc1 : (↑c1 : ℕ) = (↑a : ℕ) + (↑b : ℕ))
-  (_ : c1.bv = a.bv + b.bv)
+  (_ : c1.toBitVec = a.toBitVec + b.toBitVec)
   (c2 : U32)
-  (hc2 : c2 = core.num.U32.wrapping_sub c1 3329#u32)
+  (hc2 : c2.toBitVec = c1.toBitVec - 3329#32)
   (c3 : U32)
-  (hc3 : c3.bv = c2.bv >>> 16)
-  (h : ¬c3 = 0#u32) :
-  c3 = 65535#u32
+  (hc3 : c3.toBitVec = c2.toBitVec >>> 16)
+  (h : c3.toBitVec ≠ 0#32) :
+  c3.toBitVec = 65535#32
   := by bv_tac
 
 example
   (a : U32)
   (b : U32)
-  (h : a.val < 3329 ∧ b.val < 3329 ∨ a.val < 6658 ∧ b.val = 3329)
+  (h : a.toNat < 3329 ∧ b.toNat < 3329 ∨ a.toNat < 6658 ∧ b.toNat = 3329)
   (c1 : U32)
-  (hc1 : c1 = core.num.U32.wrapping_sub a b)
+  (hc1 : c1.toBitVec = a.toBitVec - b.toBitVec)
   (c2 : U32)
-  (hc2 : c2.bv = c1.bv >>> 16) :
-  (decide (c2 = 0#u32) || decide (c2 = 65535#u32)) = true
+  (hc2 : c2.toBitVec = c1.toBitVec >>> 16) :
+  c2.toBitVec = 0#32 ∨ c2.toBitVec = 65535#32
   := by
   bv_tac
 
 example
   (a : U32)
   (b : U32)
-  (h : a.val < 3329 ∧ b.val < 3329 ∨ a.val < 6658 ∧ b.val = 3329)
+  (h : a.toNat < 3329 ∧ b.toNat < 3329 ∨ a.toNat < 6658 ∧ b.toNat = 3329)
   (c1 : U32)
-  (hc1 : c1 = core.num.U32.wrapping_sub a b)
+  (hc1 : c1.toBitVec = a.toBitVec - b.toBitVec)
   (c2 : U32)
-  (hc2 : c2.bv = c1.bv >>> 16)
+  (hc2 : c2.toBitVec = c1.toBitVec >>> 16)
   (c3 : U32)
-  (hc3_1 : c3.val = (3329#u32 &&& c2).val)
-  (_ : c3.bv = 3329#32 &&& c2.bv)
+  (_ : c3.toBitVec = 3329#32 &&& c2.toBitVec)
   (c4 : U32)
-  (hc3 : c4 = core.num.U32.wrapping_add c1 c3) :
-  (c4.val : ZMod 3329) = (a.val : ZMod 3329) - (b.val : ZMod 3329) ∧ c4.val < 3329
+  (hc3 : c4.toBitVec = c1.toBitVec + c3.toBitVec) :
+  (c4.toBitVec + b.toBitVec) % 3329#32 = a.toBitVec % 3329#32 ∧ c4.toBitVec < 3329#32
   := by
-  bv_tac 32
+  bv_tac
 
 end Aeneas.BvTac
